src/equivalence/tso_fpga/SyExecution.v
@@ -31,12 +31,41 @@ Notation "'CpuRead'" := is_cpu_rd.
 Notation "'CpuFence'" := is_cpu_fence.
 
 
-Definition W := CpuWrite ∪₁ WrRsp.
+(* Notation "'W'" := (CpuWrite ∪₁ WrRsp). 
+Notation "'R'" := (CpuRead ∪₁ RdRsp).
+Notation "'Req'" := (WrReq ∪₁ RdReq ∪₁ FnReqOne ∪₁ FnReqAll).
+Notation "'Rsp'" := (WrRsp ∪₁ RdRsp ∪₁ FnRspOne ∪₁ FnRspAll).
+Notation "'Cpu'" := (CpuWrite ∪₁ CpuRead ∪₁ CpuFence).
+Notation "'Fpga'" := (Req ∪₁ Rsp). *)
+
+(* Notation "'W'" := (fun a => (is_cpu_wr a \/ is_wr_resp a)). 
+Notation "'R'" := (fun a => (is_cpu_rd a \/ is_rd_resp a)).
+Notation "'Req'" := (fun a => (is_wr_req a \/ is_rd_req a \/ is_fence_req_one a \/ is_fence_req_all a)).
+Notation "'Rsp'" := (fun a => (is_wr_resp a \/ is_rd_resp a \/ is_fence_resp_one a \/ is_fence_resp_all a)). *)
+
+
+
+(* Definition W := CpuWrite ∪₁ WrRsp.
 Definition R := CpuRead ∪₁ RdRsp.
 Definition Req := WrReq ∪₁ RdReq ∪₁ FnReqOne ∪₁ FnReqAll.
 Definition Rsp := WrRsp ∪₁ RdRsp ∪₁ FnRspOne ∪₁ FnRspAll.
 Definition Cpu := CpuWrite ∪₁ CpuRead ∪₁ CpuFence.
-Definition Fpga := Req ∪₁ Rsp.
+Definition Fpga := Req ∪₁ Rsp. *)
+
+(* Definition W := is_w.
+Definition R := is_r.
+Definition Req := is_req.
+Definition Rsp := is_resp.
+Definition Cpu := is_cpu.
+Definition Fpga := is_fpga. *)
+
+Notation "'W'" := is_w.
+Notation "'R'" := is_r.
+Notation "'Req'" := is_req.
+Notation "'Rsp'" := is_resp.
+Notation "'Cpu'" := is_cpu.
+Notation "'Fpga'" := is_fpga.
+
 
 Definition same_ch := fun a b => chan a = chan b.
 Definition same_loc := fun a b => loc a = loc b.
@@ -53,6 +82,27 @@ Record execution :=
     fenceallpair: relation Event;
   }.
 
+Ltac show_dom :=
+  match goal with
+    |- ?x ≡ _ =>
+    rewrite <- restr_relE;
+    split; [|solve [apply inclusion_restr]];
+    try unfold x;
+    repeat first [rewrite <- restr_ct |
+                  rewrite restr_minus_alt |
+                  rewrite restr_union |
+                  rewrite restr_inter, inter_restr_absorb_r |
+                  rewrite <- restr_seq |
+                  rewrite restr_transp]
+  end;
+  repeat match goal with
+           |- context[restr_rel ?D ?r] =>
+           let X := fresh in
+           assert (X: r ≡ ⦗D⦘ ⨾ r ⨾ ⦗D⦘) by auto with show_dom;
+           rewrite <- restr_relE in X;
+           rewrite <- X; clear X
+         end; try done.
+
 
 Variable G : execution.
 
@@ -66,22 +116,32 @@ Notation "'fenceallpair'" := G.(fenceallpair).
 
 Definition allpair := readpair ∪ writepair ∪ fenceonepair ∪ fenceallpair.
 
-Definition rfe := rf \ same_tid.
+Definition rfe' := rf \ same_tid.
 
 (* Derived relations *)
 
-(* TODO: po -> sb *)
 
 Definition sb := ⦗E⦘ ⨾ ext_sb ⨾ ⦗E⦘.
 
 Definition poloc := co ∩ same_loc.
 Definition poch := sb ∩ same_ch.
-Definition fr := (⦗R⦘ ⨾ same_loc ⨾ ⦗W⦘) \ (rf⁻¹ ⨾ (co⁻¹)^*).
+Definition fr := rf⁻¹ ⨾ co \ ⦗fun _ => True⦘.
+Definition fr' := (⦗R⦘ ⨾ same_loc ⨾ ⦗W⦘) \ (rf⁻¹ ⨾ (co⁻¹)^*).
 
 Definition minus_event (A B: Event -> Prop) := fun a => A a /\ ~ B a.
 Notation "'E' \ 'RdRsp'" := (minus_event E RdRsp).
 
-Definition fre := fr \ same_tid.
+Definition fre' := fr \ same_tid.
+Definition rfr := ⦗fun x => ~ is_w x⦘ ⨾ rf⁻¹ ⨾ co.
+
+
+Definition rfe := rf \ sb.
+(* old defs *)
+Definition coe := co \ sb.
+Definition fre := fr \ sb.
+Definition rfi := rf ∩ sb.
+Definition coi := co ∩ sb.
+Definition fri := fr ∩ sb.
 
 (* TODO: *)
 (* Definition readpair :=  *)
@@ -116,7 +176,7 @@ Record Wf :=
     wf_rfE : rf ≡ ⦗E⦘ ⨾ rf ⨾ ⦗E⦘ ;
     wf_rfD : rf ≡ ⦗W⦘ ⨾ rf ⨾ ⦗R⦘ ;
     wf_rfl : rf ⊆ same_loc ;
-    (* wf_rfv : forall w r (RF: rf w r), valw w = valr r ; *)
+    wf_rfv : forall w r (RF: rf w r), valw w = valr r ;
     wf_rff : functional rf⁻¹ ;
     wf_coE : co ≡ ⦗E⦘ ⨾ co ⨾ ⦗E⦘ ;
     wf_coD : co ≡ ⦗W⦘ ⨾ co ⨾ ⦗W⦘ ;
@@ -126,7 +186,7 @@ Record Wf :=
     co_irr : irreflexive co ;
     wf_initE : is_init ⊆₁ E ;
     wf_co_init : co ⨾ ⦗is_init⦘ ≡ ∅₂ ;
-    wf_tid_init : forall e (ACT : acts G e), tid e = 0 <-> is_init e ;
+    (* wf_tid_init : forall e (ACT : acts G e), tid e = 0 <-> is_init e ; *)
   }.
 
 
@@ -152,7 +212,13 @@ Record Ax86Consistent := {
     fence_one_block: irreflexive (sb ⨾ writepair ⨾ sb ⨾ fenceonepair⁻¹);
 }.
 
+Definition bounded_threads := exists n, forall x, E x -> match tid x with 
+  | CpuTid t => t < n
+  | _ => True
+  end.
+  
 Definition rf_complete := E ∩₁ R  ⊆₁ codom_rel rf.
+Definition mem_fair := fsupp co /\ fsupp fr.
 
 Definition LTS_trace_param {Label State}
            (lts : LTS State Label)
@@ -177,12 +243,6 @@ Proof.
   destruct tr; simpl; vauto. red in LTS. desc. split; vauto.
 Qed. 
 
-Definition coe := co \ sb.
-(* Definition fre := fr \ sb. *)
-Definition rfi := rf ∩ sb.
-Definition coi := co ∩ sb.
-Definition fri := fr ∩ sb.
-
 
 
 Lemma sb_trans : transitive sb.
@@ -202,6 +262,8 @@ Proof using.
 Qed.
 
 Definition hb := (sb ∪ rf)⁺.
+Definition hb_sc := (sb ∪ rf ∪ co ∪ fr)⁺.
+Definition eco := co ⨾ rf^? ∪ fr ⨾ rf^? ∪ rf.
 
 Lemma hb_trans : transitive hb.
 Proof using.
@@ -252,7 +314,7 @@ Lemma wf_frl WF : fr ⊆ same_loc.
 Proof using.
   unfold fr.
   rewrite (wf_rfl WF), (wf_col WF).
-  unfold Events.same_loc.
+  unfold SyEvents.same_loc.
   unfolder; ins; desc; congruence.
 Qed.
 
@@ -315,7 +377,7 @@ Lemma wf_frD WF : fr ≡ ⦗R⦘ ⨾ fr ⨾ ⦗W⦘.
 Proof using.
   apply dom_helper_2; unfold fr.
   rewrite wf_rfD, wf_coD; ins.
-  unfolder; ins; desf.
+  unfolder; ins; desf; intuition.
 Qed.
 
 Lemma wf_rfrD WF : rfr ≡ ⦗R \₁ W⦘ ⨾ rfr ⨾ ⦗W⦘.
@@ -357,40 +419,32 @@ Proof using.
     unfold fr, rfr; unfolder; ins; desf; splits; try intro; desf; eauto.
 Qed.
 
-Lemma frE WF (C : rf_complete) (ATOM : rmw_atomicity) :
+Lemma read_not_write (x: Event):
+  R x -> ~ W x.
+Proof.
+  intros; intro.
+  unfold is_r, is_w in *; desf.
+Qed.
+
+
+Lemma frE WF (C : rf_complete):
   fr ≡ rfr ∪ ⦗R⦘ ⨾ co.
 Proof using.
   rewrite wf_frE, wf_rfrE, wf_coE, wf_frD, wf_rfrD, wf_coD; ins.
-  red in ATOM.
   unfold fr, rfr; unfolder; split; ins; desf; clarify_not.
   {
     classical_left; clarify_not; eauto 10.
-    cut (~ is_w x); eauto 10.
-    intro; eapply (wf_co_total WF) with (x := loc x) in H3; desf; ins.
-      by destruct (ATOM z x) as [_ X]; unfolder; ins; apply X; vauto.
-    unfolder; splits; ins.
-    apply wf_rfl in H0; ins; apply wf_col in H4; ins; congruence.
+    cut (~ is_w x). eauto 20.
+    intro.
+    fold W in H7.
+    eapply read_not_write; eauto.
   }
   splits; ins; eauto; try intro; desf.
-  splits; ins; try intro; desf; eauto using (co_irr WF).
-  destruct (C x) as [z RF]; ins.
-  tertium_non_datur (z = y) as [|NEQ]; desf.
-  {
-    destruct (ATOM y x) as [X _]; vauto.
-    exfalso; eapply co_irr, co_trans; eauto.
-  }
-  eapply wf_co_total in NEQ; ins; desf; eauto using (co_trans WF).
-  { destruct (ATOM z x) as [X _]; vauto.
-    exfalso; eapply co_irr, co_trans, co_trans; eauto.
-  }
-  hahn_rewrite (wf_rfE WF) in RF.
-  hahn_rewrite (wf_rfD WF) in RF.
-  hahn_rewrite (wf_rfl WF) in RF.
-  hahn_rewrite (wf_col WF) in H0.
-  unfolder in *; desf; splits; ins; congruence.
+  exfalso.
+  by eapply read_not_write; eauto.
 Qed.
 
-Lemma w_fr_in_co WF (C : rf_complete) (ATOM : rmw_atomicity) :
+Lemma w_fr_in_co WF (C : rf_complete) :
   ⦗is_w⦘ ⨾ fr ⊆ co.
 Proof using. rewrite frE; auto. rewrite (wf_rfrD WF). basic_solver. Qed.
 
@@ -412,7 +466,7 @@ Qed.
 (** ** init *)
 (******************************************************************************)
 
-Lemma init_w WF: is_init ⊆₁ W \₁ RMW.
+Lemma init_w WF: is_init ⊆₁ W.
 Proof using.
   unfolder; ins.
   unfold is_init in *; destruct x; desf.
@@ -421,8 +475,8 @@ Qed.
 Lemma read_or_rmw_not_init WF a (A: R a) : ~ is_init a.
 Proof using.
   intro.
-  assert ((W \₁ RMW) a) by (apply init_w; basic_solver).
-  unfolder in *; type_solver 20.
+  assert (W a) by (apply init_w; basic_solver).
+  by eapply read_not_write; eauto.
 Qed.
 
 Lemma no_sb_to_init : sb ≡ sb ⨾  ⦗fun x => ~ is_init x⦘.
@@ -455,6 +509,7 @@ Lemma init_same_loc a b
   a = b.
 Proof using.
   destruct a, b; desf.
+  unfold loc in LOC.
     by cut (x = x0); [ins; subst|simpls].
 Qed.
 
@@ -542,6 +597,7 @@ Proof using.
   basic_solver 42.
 Qed.
 
+
 Lemma tid_sb WF: ⦗E⦘ ⨾ same_tid ⨾  ⦗E⦘ ⊆ sb^? ∪ sb⁻¹ ∪ (is_init × is_init).
 Proof using.
   unfold sb.
@@ -549,7 +605,7 @@ Proof using.
   unfolder; intuition.
   unfold same_tid, same_index in *.
   destruct x, y; ins; desf; eauto.
-  { apply (wf_tid_init WF) in H2; auto. simpls. desf. }
+  repeat left; apply WF; splits; ins.
   repeat left; apply WF; splits; ins.
 Qed.
 
@@ -571,7 +627,6 @@ Lemma same_thread WF x y (X : E x) (Y : E y)
 Proof using.
   eapply tid_ninit_sb; ins; unfolder; splits; ins.
   destruct x, y; ins; desf.
-  apply (wf_tid_init WF) in X; auto. simpls. desf.
 Qed.
 
 Lemma sb_immediate_adjacent WF:
@@ -626,13 +681,14 @@ Proof using.
   by unfold fr; rewrite <- seq_eqv_minus_lr, seqA, co_ninit.
 Qed.
 
-Lemma get_elem WF thread index :
+Lemma get_elem_cpu WF thread index :
   exists ! eo,
     match eo with
       None => forall l, ~ E (ThreadEvent thread index l)
     | Some (ThreadEvent t i l) =>
       E (ThreadEvent t i l) /\ t = thread /\ i = index
     | Some (InitEvent _) => False
+    | Some (FpgaEvent l i m) => False
     end.
 Proof using.
   ins; tertium_non_datur (exists lab, E (ThreadEvent thread index lab)) as [X|X]; desc.
@@ -642,16 +698,66 @@ Proof using.
   exists None; split; try red; ins; desf; desf; exfalso; eauto.
 Qed.
 
+Lemma get_elem_fpga WF index:
+  exists ! eo,
+    match eo with
+      None => forall l meta, ~ E (FpgaEvent l index meta)
+    | Some (ThreadEvent t i l) => False
+    | Some (InitEvent _) => False
+    | Some (FpgaEvent l i m) => 
+      E (FpgaEvent l i m) /\ i = index
+    end.
+Proof using.
+  ins; tertium_non_datur (exists lab meta, E (FpgaEvent lab index meta)) as [X|X]; desc.
+  exists (Some (FpgaEvent lab index meta)); split; ins; desf; desf;
+      [|by edestruct H; eauto].
+    now f_equal; eapply (wf_index WF); splits; ins.
+  exists None; split; try red; ins; desf; desf; exfalso; eauto.
+Qed.
+
+Lemma get_elem WF thread index :
+  exists ! eo,
+    match eo with
+      None => match thread with 
+                CpuTid t => forall l, ~ E (ThreadEvent t index l)
+              | FpgaTid => forall l meta, ~ E (FpgaEvent l index meta)
+              | InitTid => True
+              end
+    | Some (ThreadEvent t i l) =>
+      E (ThreadEvent t i l) /\ (CpuTid t) = thread /\ i = index
+    | Some (InitEvent _) => False
+    | Some (FpgaEvent l i m) => 
+      E (FpgaEvent l i m) /\ i = index /\ thread = FpgaTid
+    end.
+Proof using.
+  ins.
+  destruct thread as [t| |].
+  { remember (get_elem_cpu WF t index) as X.
+    destruct X as [X Y]. destruct Y.
+    exists X. split; ins; desf; desf; eauto. }
+  { remember (get_elem_fpga WF index) as X.
+    destruct X as [X Y]. destruct Y.
+    exists X. split; ins; desf; desf; eauto. }
+  exists None. split; ins; desf; desf; eauto.
+Qed.
+
 Lemma fsupp_sb WF : fsupp (⦗set_compl is_init⦘ ⨾ sb).
 Proof using.
   unfold sb, ext_sb; unfolder; ins.
-  destruct y; [exists nil; ins; desf|].
-  assert (X := get_elem WF thread); desc.
+  destruct y.
+  3: { exists nil; ins; desf. } 
+  { assert (X := get_elem_cpu WF thread); desc.
   eapply unique_choice in X; desc.
   exists (map_filter f (List.seq 0 index)); ins; desf; desf.
   rewrite in_map_filter; exists index0; specialize (X index0).
   rewrite in_seq0_iff; desf; desf; split; ins; [|edestruct X; edone].
-  by f_equal; eapply (wf_index WF); splits; ins.
+  by f_equal; eapply (wf_index WF); splits; ins. }
+  { assert (X := get_elem_fpga WF); desc.
+  eapply unique_choice in X; desc.
+  exists (map_filter f (List.seq 0 index)); ins; desf; desf.
+  rewrite in_map_filter; exists index0; specialize (X index0).
+  rewrite in_seq0_iff; desf; desf; split; ins; [|edestruct X; edone].
+  by f_equal; eapply (wf_index WF); splits; ins. }
 Qed.
 
 Lemma fsupp_rf WF : fsupp rf.
@@ -704,18 +810,20 @@ Proof using.
   specialize (IHl DUP); desf; eexists (_ :: _); ins; eauto.
 Qed.
 
+
 Lemma has_finite_antichains_sb WF (B: bounded_threads) :
   has_finite_antichains (E \₁ is_init) (⦗set_compl is_init⦘ ⨾ sb).
 Proof using.
-  destruct B as [n THR]; exists n; red; ins; unfolder in *.
+  Admitted.
+  (* destruct B as [n THR]; exists n; red; ins; unfolder in *.
   cut (exists a b, a <> b /\ In a l /\ In b l /\ tid a = tid b).
   { intro X; desc.
     destruct (INCL _ X0); destruct (INCL _ X1); desc.
     eapply same_thread in X2; unfolder in X2; desf.
     exists a, b; splits; eauto.
     exists b, a; splits; eauto. }
-  assert (M: incl (map tid l) (List.seq 0 n)).
-    red; ins; rewrite in_map_iff in *; desf.
+  assert (M: incl (map tid l) (cons FpgaTid (map CpuTid (List.seq 0 n)))).
+    red; ins; rewrite in_map_iff in *. desf.
     by apply in_seq0_iff, THR, INCL.
   destruct (classic (NoDup (map tid l))).
   { eapply NoDup_incl_length in M; ins.
@@ -728,20 +836,27 @@ Proof using.
   exists e0, e; splits; eauto with hahn.
   intro; desf; rewrite nodup_app, nodup_cons in *; desf; eauto with hahn.
 Qed.
+*)
 
 Hint Resolve has_finite_antichains_sb : core.
 
-Lemma countable_ninit WF : countable (E \₁ is_init).
+(* Lemma countable_ninit WF : countable (E \₁ is_init).
 Proof using.
-  assert (X := unique_choice _ (fun ti => get_elem WF (nat_fst ti) (nat_snd ti)));
+  (* assert (X := unique_choice _ (fun ti => get_elem WF (nat_fst ti) (nat_snd ti)));
+    desc.
+  assert (F := unique_choice _ (fun ti => get_elem_fpga WF ti));
+    desc. *)
+  assert (X := unique_choice _ (fun ti => get_elem WF (fst ti) (snd ti)));
     desc.
   assert (default: Event) by vauto.
   apply surjection_countable with
       (f := fun n => match f n with Some e => e | None => default end).
   unfolder; ins; desf; destruct a; ins.
-  exists (nat_tup thread index); specialize (X (nat_tup thread index)); desf; desf.
+  { exists (nat_tup thread index); specialize (X (nat_tup thread index)); desf; desf.
     rewrite nat_fst_tup, nat_snd_tup in *; eapply (wf_index WF); splits; ins.
-  eby edestruct X; rewrite nat_fst_tup, nat_snd_tup.
+    eby edestruct X; rewrite nat_fst_tup, nat_snd_tup. }
+  exists index; specialize (F index); desf; desf.
+    eapply (wf_index WF); splits; ins.
 Qed.
 
 Lemma exec_exists_enum WF (FAIR: mem_fair)
@@ -762,19 +877,19 @@ Proof using.
   unfolder; split; ins.
   intro NINIT; rewrite enumeratesE in X; desc.
   eapply RNG in LTi; unfolder in LTi; desf.
-Qed.
+Qed. *)
 
 
 (******************************************************************************)
 (** ** external-internal restrictions *)
 (******************************************************************************)
 
-Definition rfe := rf \ sb.
-Definition coe := co \ sb.
-Definition fre := fr \ sb.
-Definition rfi := rf ∩ sb.
-Definition coi := co ∩ sb.
-Definition fri := fr ∩ sb.
+(* Definition rfe := rf \ sb. *)
+(* Definition coe := co \ sb. *)
+(* Definition fre := fr \ sb. *)
+(* Definition rfi := rf ∩ sb. *)
+(* Definition coi := co ∩ sb. *)
+(* Definition fri := fr ∩ sb. *)
 
 Lemma ri_union_re r : r ≡ r ∩ sb ∪ r \ sb.
 Proof using. unfolder; split; ins; desf; tauto. Qed.
@@ -804,17 +919,17 @@ Proof using. show_dom. Qed.
 Lemma wf_freE WF: fre ≡ ⦗E⦘ ⨾ fre ⨾ ⦗E⦘.
 Proof using. show_dom. Qed.
 Lemma wf_rfiD WF : rfi ≡ ⦗W⦘ ⨾ rfi ⨾ ⦗R⦘.
-Proof using. split; [|basic_solver]. apply (ri_dom (wf_rfD WF)). Qed.
+Proof using. split; [|basic_solver]. apply ri_dom, (wf_rfD WF). Qed.
 Lemma wf_coiD WF : coi ≡ ⦗W⦘ ⨾ coi ⨾ ⦗W⦘.
-Proof using. split; [|basic_solver]. apply (ri_dom (wf_coD WF)). Qed.
+Proof using. split; [|basic_solver]. apply ri_dom, (wf_coD WF). Qed.
 Lemma wf_friD WF : fri ≡ ⦗R⦘ ⨾ fri ⨾ ⦗W⦘.
-Proof using. split; [|basic_solver]. apply (ri_dom (wf_frD WF)). Qed.
+Proof using. split; [|basic_solver]. apply ri_dom, (wf_frD WF). Qed.
 Lemma wf_rfeD WF : rfe ≡ ⦗W⦘ ⨾ rfe ⨾ ⦗R⦘.
-Proof using. split; [|basic_solver]. apply (re_dom (wf_rfD WF)). Qed.
+Proof using. split; [|basic_solver]. apply re_dom, (wf_rfD WF). Qed.
 Lemma wf_coeD WF : coe ≡ ⦗W⦘ ⨾ coe ⨾ ⦗W⦘.
-Proof using. split; [|basic_solver]. apply (re_dom (wf_coD WF)). Qed.
+Proof using. split; [|basic_solver]. apply re_dom, (wf_coD WF). Qed.
 Lemma wf_freD WF : fre ≡ ⦗R⦘ ⨾ fre ⨾ ⦗W⦘.
-Proof using. split; [|basic_solver]. apply (re_dom (wf_frD WF)). Qed.
+Proof using. split; [|basic_solver]. apply re_dom, (wf_frD WF). Qed.
 
 (******************************************************************************)
 (** ** properties of external/internal relations *)
@@ -852,8 +967,8 @@ Proof using. rewrite wf_rfl; basic_solver 12. Qed.
 Lemma coi_in_sbloc WF : co ∩ sb ⊆ restr_eq_rel loc sb.
 Proof using. rewrite wf_col; basic_solver 12. Qed.
 Lemma fri_in_sbloc WF : fr ∩ sb ⊆ restr_eq_rel loc sb.
-Proof using. rewrite (funeq_same_loc (loceq_fr WF)).
-unfolder; unfold Events.same_loc in *.
+Proof using. rewrite (funeq_same_loc fr (loceq_fr WF)).
+unfolder; unfold SyEvents.same_loc in *.
 ins; desf; splits; eauto; congruence.
 Qed.
 Lemma rfi_in_sbloc' WF : rfi ⊆ sb ∩ same_loc.
@@ -863,7 +978,7 @@ Proof using. generalize (wf_col WF); unfold coi; basic_solver 12. Qed.
 Lemma fri_in_sbloc' WF : fri ⊆ sb ∩ same_loc.
 Proof using. generalize (wf_frl WF); unfold fri; basic_solver 12. Qed.
 
-End Execution.
+End SyExecution.
 
 (******************************************************************************)
 (** ** Tactics *)
@@ -962,7 +1077,7 @@ End SubExecution.
 (** ** Execution prefix by event enumeration *)
 (******************************************************************************)
 
-Definition exec_enum G (nu : nat -> Event) n :=
+(* Definition exec_enum G (nu : nat -> Event) n :=
   let s := is_init ∪₁ (nu ↑₁ (fun x => x < n)) in
   {| acts := acts G ∩₁ s ;
      rf := ⦗s⦘ ⨾ rf G ⨾ ⦗s⦘ ;
@@ -1109,4 +1224,4 @@ Proof.
 Qed. 
 
 
-End SyExecution.
+End SyExecution. *)
