src/equivalence/tso_fpga/SyLemmas.v
@@ -37,9 +37,9 @@ Hypothesis (TSO_FAIR: TSO_fair tr states).
 Definition Ecpu := fun e => trace_elems tr (EventLab e) /\ is_cpu e.
 Definition Efpga := fun e => trace_elems tr (EventLab e) /\ is_fpga e.
 Definition Eninit := fun e => trace_elems tr (EventLab e).
-Hypothesis BOUNDED_THREADS: exists n, forall e, Eninit e -> tid e < n.
+(* Hypothesis BOUNDED_THREADS: exists n, forall e, Eninit e -> tid e < n.
 Hypothesis NO_TID0: forall e, is_cpu e -> tid e <> 0. 
-Hypothesis NO_TID1: forall e, is_cpu e -> tid e <> 1.
+Hypothesis NO_TID1: forall e, is_cpu e -> tid e <> 1. *)
 
 Definition EG := is_init ∪₁ Eninit.
 
@@ -55,13 +55,8 @@ Defined.
 
 Lemma not_same_tid_cpu_fpga e1 e2 (E1: is_cpu e1) (E2: is_fpga e2) (EQ: tid e1 = tid e2): False.
 Proof.
-  assert (tid e1 <> 1). eapply NO_TID1. eauto.
-  assert (tid e2 = 1).
-  {
-    unfold tid.
-    destruct e2; auto;unfold Efpga in E2; desc; unfold is_fpga in E2; done.
-  }
-  lia.
+  unfolder'.
+  desf.
 Qed.
 
 
@@ -81,6 +76,30 @@ Proof.
   destruct (constructive_indefinite_description _ _). desc.
   rewrite <- a0. by apply trace_nth_indep. 
 Qed. 
+
+Lemma nth_not_default_found x (l: list SyLabel) d (NOT_DEF: (nth x l d) <> d):
+  x < length l.
+Proof.
+  generalize dependent x.
+  induction l; ins.
+  { unfold nth in NOT_DEF; desf. }
+  simpl in NOT_DEF.
+  destruct x.
+  { simpl; lia. }
+  remember (IHl x NOT_DEF); lia.
+Qed.
+
+Lemma not_default_found x (NOT_DEF: (trace_labels x) <> def_lbl): 
+  NOmega.lt_nat_l x (trace_length tr).
+Proof.
+  unfold trace_labels in *.
+  unfold trace_nth in *.
+  destruct tr.
+  2: vauto.
+  unfold NOmega.lt_nat_l.
+  unfold trace_length.
+  apply nth_not_default_found in NOT_DEF; auto.
+Qed.
 
 Lemma trace_index_simpl' e (ENINIT: Eninit e):
   trace_labels (trace_index e) = EventLab e.
@@ -124,6 +143,7 @@ Proof.
       destruct WF as [WF_cpu WF_fpga].
       forward eapply (@WF_cpu x0 x def_lbl thread index0 index e0 e); auto.
       lia.
+      unfolder'. vauto.
     }
     {
       simpl in H0. desc. split; auto.
@@ -188,6 +208,7 @@ Proof.
   }
 Qed. 
 
+
 Lemma tb_SPO: strict_total_order Eninit trace_before.
 Proof.
   red. split.
@@ -197,6 +218,7 @@ Proof.
   pose proof (Nat.lt_trichotomy (trace_index a) (trace_index b)). des; auto.
   by apply ti_inj in H.
 Qed.
+
 
 Definition is_init' e :=
   match e with
@@ -214,6 +236,7 @@ Definition is_init' e :=
 (*   end. *)
 Definition count_upto S bound :=
   length (filterP S (map (fun i : nat => trace_nth i tr def_lbl) (List.seq 0 bound))).
+
 
 Definition state_before_event e := states (trace_index e). 
 
@@ -233,7 +256,7 @@ Proof. unfold check. destruct (excluded_middle_informative (S elt)); vauto. Qed.
 
 
 Lemma buffer_same_transition st1 st2 lbl thread (STEP: TSOFPGA_step st1 lbl st2)
-      (OTHER: lbl_thread_opt lbl <> Some thread):
+      (OTHER: lbl_thread lbl <> CpuTid thread):
   cpu_bufs (st1) thread = cpu_bufs (st2) thread. 
 Proof.
   destruct st1 as [mem1 buf1]. destruct st2 as [mem2 buf2]. simpl.
@@ -396,12 +419,12 @@ Ltac liaW no := (destruct no; [done|simpl in *; lia]).
 
 Lemma buffer_size_inv st1 st2 lbl thread (STEP: TSOFPGA_step st1 lbl st2):
 length (cpu_bufs st1 thread) +
-check (cpu_write' ∩₁ in_thread thread) lbl =
-check (is_cpu_prop ∩₁ in_thread thread) lbl +
+check (cpu_write' ∩₁ in_cpu_thread thread) lbl =
+check (is_cpu_prop ∩₁ in_cpu_thread thread) lbl +
 length (cpu_bufs st2 thread).
 Proof.
 destruct st1 as [mem1 buf1]. destruct st2 as [mem2 buf2]. simpl.
-destruct (classic (lbl_thread_opt lbl = Some thread)) as [EQ | NEQ] .
+destruct (classic (lbl_thread lbl = CpuTid thread)) as [EQ | NEQ] .
 2: { forward eapply buffer_same_transition as SAME_BUF; eauto. simpl in SAME_BUF.
       rewrite SAME_BUF. 
       repeat rewrite check0; [lia| |].
@@ -421,9 +444,16 @@ inversion STEP; subst; simpl in EQ; inv EQ.
 Qed. 
 
 
+
 Definition is_store_ups (upsE: (UpstreamEntry * Mdata)) :=
   match upsE with
   | ((store_up _ _), _) => true
+  | _ => false
+end.
+
+Definition is_read_ups (upsE: (UpstreamEntry * Mdata)) :=
+  match upsE with
+  | ((read_up _), _) => true
   | _ => false
 end.
 
@@ -469,20 +499,65 @@ inversion STEP; subst; simpl in EQ; inv EQ.
 }
 Qed.
 
+(* TODO: Delete
+Lemma upstream_read_size_inv st1 st2 lbl chan (STEP: TSOFPGA_step st1 lbl st2):
+length (filter is_read_ups (up_bufs st1 chan)) +
+check (fpga_read_resp' ∩₁ in_chan chan) lbl =
+check (fpga_mem_read' ∩₁ in_chan chan) lbl +
+length (filter is_read_ups (up_bufs st2 chan)).
+Proof.
+destruct st1 as [wp1 rp1 up_buf1 db1 shm1 cpu_b1]. destruct st2 as [wp2 rp2 up_buf2 db2 shm2 cpu_b2]. simpl.
+destruct (classic (lbl_chan_opt lbl = Some chan)) as [EQ | NEQ] .
+2: { forward eapply upstream_same_transition as SAME_BUF; eauto. simpl in SAME_BUF.
+      rewrite SAME_BUF. 
+      repeat rewrite check0; [lia| |].
+      all: apply set_compl_inter; right; vauto. }
+inversion STEP; subst; simpl in EQ; inv EQ.
+ all: try (repeat rewrite check0; [lia| |]; apply set_compl_inter; left; vauto).
+{ rewrite check0.
+  2: { unfolder'. simpl. intuition. }
+  rewrite check0.
+  2: { unfolder'. simpl. intuition. }
+  rewrite upds. rewrite filter_app. rewrite length_app. by simpl. }
+{ rewrite upds. rewrite UPSTREAM. simpl.
+  rewrite check0; [| unfolder'; simpl; intuition].
+  rewrite check0; [| unfolder'; simpl; intuition].
+  vauto. }
+{ 
+  rewrite check1. 2: { unfolder'. simpl. intuition. }
+  rewrite check0; [|unfolder'; simpl; intuition]). 
+
+}
+  rewrite upds. rewrite filter_app. rewrite length_app. simpl.
+  rewrite check0; [| unfolder'; simpl; intuition].
+  lia.
+}
+{
+  rewrite check0.
+  2: { unfolder'. simpl. intuition. }
+  rewrite check0.
+  2: { unfolder'. simpl. intuition. }
+  rewrite UPSTREAM.
+  rewrite upds. 
+  simpl.
+  lia.
+}
+Qed. *)
+
 Lemma buffer_size_cpu thread i (DOM: NOmega.le (NOnum i) (trace_length tr)):
-  count_upto (cpu_write' ∩₁ in_thread thread) i = count_upto (is_cpu_prop ∩₁ in_thread thread) i + length (cpu_bufs (states i) thread).
+  count_upto (cpu_write' ∩₁ in_cpu_thread thread) i = count_upto (is_cpu_prop ∩₁ in_cpu_thread thread) i + length (cpu_bufs (states i) thread).
 Proof.
   induction i.
   { simpl. unfold count_upto. rewrite seq0. simpl.
     pose proof TS0 as TS0. simpl in TS0. by rewrite <- TS0. }
   remember (states (S i)) as s. simpl.
   unfold count_upto. rewrite !seqS, !Nat.add_0_l, !map_app, !filterP_app, !length_app. simpl.
-  fold (count_upto (cpu_write' ∩₁ in_thread thread) i).
-  fold (count_upto (is_cpu_prop ∩₁ in_thread thread) i).
+  fold (count_upto (cpu_write' ∩₁ in_cpu_thread thread) i).
+  fold (count_upto (is_cpu_prop ∩₁ in_cpu_thread thread) i).
   specialize_full IHi.
   { apply NOmega.le_trans with (m := NOnum (S i)); vauto. } 
-  fold (check (cpu_write' ∩₁ in_thread thread) (trace_nth i tr def_lbl)). 
-  fold (check (is_cpu_prop ∩₁ in_thread thread) (trace_nth i tr def_lbl)). 
+  fold (check (cpu_write' ∩₁ in_cpu_thread thread) (trace_nth i tr def_lbl)). 
+  fold (check (is_cpu_prop ∩₁ in_cpu_thread thread) (trace_nth i tr def_lbl)). 
   remember (states i) as st_prev.
   rewrite IHi.
   rewrite <- !Nat.add_assoc.
@@ -494,7 +569,7 @@ Proof.
 Qed. 
 
 
-Lemma buffer_size_fpga chan i (DOM: NOmega.le (NOnum i) (trace_length tr)):
+Lemma buffer_size_upstream_write chan i (DOM: NOmega.le (NOnum i) (trace_length tr)):
   count_upto (fpga_write' ∩₁ in_chan chan) i = 
   count_upto (is_fpga_prop ∩₁ in_chan chan) i + length (filter is_store_ups (up_bufs (states i) chan)).
 Proof.
@@ -519,6 +594,11 @@ Proof.
   forward eapply (TSi i) with (d := def_lbl) as TSi; vauto.
 Qed.
 
+Lemma buffer_size_upstream_read chan i (DOM: NOmega.le (NOnum i) (trace_length tr)):
+  count_upto (fpga_read_resp' ∩₁ in_chan chan) i + length (filter is_read_ups (up_bufs (states i) chan))= 
+  count_upto (fpga_mem_read' ∩₁ in_chan chan) i .
+Proof.
+  Admitted.
 
 Lemma EXACT_CHAN_PROPS chan:
   trace_length (trace_filter (fpga_write' ∩₁ in_chan chan) tr) =
@@ -621,9 +701,7 @@ Definition same_chan x y :=
   let chan := lbl_chan_opt x in
   chan = lbl_chan_opt y /\ chan <> None. 
 
-Definition same_thread x y :=
-  let thread := lbl_thread_opt x in
-  thread = lbl_thread_opt y /\ thread <> None.
+Definition same_thread x y := lbl_thread x = lbl_thread y.
 
 Lemma write2prop_fpga_lem w
     (* (DOM: NOmega.lt_nat_l w (trace_length tr)) *)
@@ -654,41 +732,82 @@ pose proof sim_subtraces_conv as TMP. specialize_full TMP.
 desc. exists j. splits; vauto.
 Qed.
 
+Lemma filter_eq_pred (l: list SyLabel) (f g: SyLabel -> Prop): (forall x, (f x <-> g x)) -> filterP f l = filterP g l.
+Proof. 
+  induction l; vauto.
+  ins.
+  erewrite IHl; vauto.
+  destruct (excluded_middle_informative (f a)) as [FA | NFA].
+  { destruct (H a) as [LR RL].
+    desf.
+    exfalso; apply (n (LR FA)).
+  }
+  { destruct (H a) as [LR RL].
+    desf.
+    exfalso; apply (NFA (RL g0)).
+  }
+Qed.
+
+Lemma count_same_chan_in_chan (c: Chan) (l: SyLabel) (InChan: in_chan c l) pred i
+  : count_upto (pred ∩₁ same_chan l) i = count_upto (pred ∩₁ in_chan c) i.
+Proof.
+  unfold count_upto.
+  remember ((map
+  (fun i0 : nat =>
+   trace_nth i0 tr def_lbl)
+  (List.seq 0 i))) as lst.
+  remember (pred ∩₁ same_chan l) as p1.
+  remember (pred ∩₁ in_chan c) as p2.
+  assert (forall x, p1 x <-> p2 x).
+  { ins.
+    assert (same_chan l x <-> in_chan c x). {
+      unfold same_chan in *.
+      unfold in_chan in *.
+      rewrite InChan.
+      split; ins; desf.
+    }
+    vauto.
+    unfold set_inter in *.
+    intuition.
+  }
+  by erewrite (filter_eq_pred lst p1 p2 H).
+Qed.
+
 
 Lemma EXACT_CPU_PROPS thread:
-  trace_length (trace_filter (cpu_write' ∩₁ in_thread thread) tr) =
-  trace_length (trace_filter (is_cpu_prop ∩₁ in_thread thread) tr).
+  trace_length (trace_filter (cpu_write' ∩₁ in_cpu_thread thread) tr) =
+  trace_length (trace_filter (is_cpu_prop ∩₁ in_cpu_thread thread) tr).
 Proof.
-remember (trace_length (trace_filter (cpu_write' ∩₁ in_thread thread) tr)) as len_writes.
-remember (trace_length (trace_filter (is_cpu_prop ∩₁ in_thread thread) tr)) as len_props. 
+remember (trace_length (trace_filter (cpu_write' ∩₁ in_cpu_thread thread) tr)) as len_writes.
+remember (trace_length (trace_filter (is_cpu_prop ∩₁ in_cpu_thread thread) tr)) as len_props. 
 pose proof (NOmega_lt_trichotomy len_writes len_props). des; auto.
 { exfalso. destruct len_writes as [|n_writes]; auto.
-  forward eapply (trace_nth_filter (is_cpu_prop ∩₁ in_thread thread) tr n_writes def_lbl) as [extra_prop_pos [DOM_EP [MATCH_PROP COUNT_PROPS]]].
+  forward eapply (trace_nth_filter (is_cpu_prop ∩₁ in_cpu_thread thread) tr n_writes def_lbl) as [extra_prop_pos [DOM_EP [MATCH_PROP COUNT_PROPS]]].
   { vauto. }
-  fold (count_upto (is_cpu_prop ∩₁ in_thread thread) extra_prop_pos) in COUNT_PROPS.
-  forward eapply (filter_ends tr (cpu_write' ∩₁ in_thread thread) def_lbl) as [w_bound [DOM_WB WRITES_BOUND]]. 
+  fold (count_upto (is_cpu_prop ∩₁ in_cpu_thread thread) extra_prop_pos) in COUNT_PROPS.
+  forward eapply (filter_ends tr (cpu_write' ∩₁ in_cpu_thread thread) def_lbl) as [w_bound [DOM_WB WRITES_BOUND]]. 
   { by rewrite <- Heqlen_writes. }
   set (bound := max (extra_prop_pos + 1) w_bound).     
   forward eapply (buffer_size_cpu thread bound) as BUF_SIZE.
   { destruct tr; auto. simpl in *. subst bound.
     apply NPeano.Nat.max_lub_iff. split; lia. }
   simpl in BUF_SIZE. remember (states bound) as st.
-  cut (count_upto (cpu_write' ∩₁ in_thread thread) bound <= n_writes /\
-        count_upto (is_cpu_prop ∩₁ in_thread thread) bound > n_writes).
+  cut (count_upto (cpu_write' ∩₁ in_cpu_thread thread) bound <= n_writes /\
+        count_upto (is_cpu_prop ∩₁ in_cpu_thread thread) bound > n_writes).
     
   { ins. desc. lia. }
   split.
-  { cut (NOmega.le (NOnum (count_upto (cpu_write' ∩₁ in_thread thread) bound)) (NOnum n_writes)).
+  { cut (NOmega.le (NOnum (count_upto (cpu_write' ∩₁ in_cpu_thread thread) bound)) (NOnum n_writes)).
     { ins. }
     rewrite Heqlen_writes. unfold count_upto. apply count_le_filter.
     simpl. destruct (trace_length tr); vauto.
     subst bound. apply Nat.max_lub_iff. simpl in *. split; lia. }
-  unfold gt. apply Nat.lt_le_trans with (m := count_upto (is_cpu_prop ∩₁ in_thread thread) (extra_prop_pos + 1)).
+  unfold gt. apply Nat.lt_le_trans with (m := count_upto (is_cpu_prop ∩₁ in_cpu_thread thread) (extra_prop_pos + 1)).
   { rewrite COUNT_PROPS.
     rewrite Nat.add_1_r, count_upto_next.
     rewrite check1; [lia| ].
     unfold trace_labels. rewrite <- MATCH_PROP.
-    forward eapply (trace_nth_in (trace_filter (is_cpu_prop ∩₁ in_thread thread) tr) n_writes) with (d := def_lbl) as IN_FILTER. 
+    forward eapply (trace_nth_in (trace_filter (is_cpu_prop ∩₁ in_cpu_thread thread) tr) n_writes) with (d := def_lbl) as IN_FILTER. 
     { rewrite <- Heqlen_props. vauto. }
     vauto. 
     apply trace_in_filter in IN_FILTER. by desc. }
@@ -696,9 +815,9 @@ pose proof (NOmega_lt_trichotomy len_writes len_props). des; auto.
 exfalso. 
 destruct len_props as [|n_props]; auto.
 
-forward eapply (trace_nth_filter (cpu_write' ∩₁ in_thread thread) tr n_props def_lbl) as [extra_write_pos [DOM_EW [MATCH_WRITE COUNT_WRITES]]].
+forward eapply (trace_nth_filter (cpu_write' ∩₁ in_cpu_thread thread) tr n_props def_lbl) as [extra_write_pos [DOM_EW [MATCH_WRITE COUNT_WRITES]]].
 { vauto. }
-fold (count_upto (cpu_write' ∩₁ in_thread thread) extra_write_pos) in COUNT_WRITES.
+fold (count_upto (cpu_write' ∩₁ in_cpu_thread thread) extra_write_pos) in COUNT_WRITES.
 set (enabled st := exists st', TSOFPGA_step st (CpuFlush thread) st').
 assert (forall i (GE: i >= (extra_write_pos + 1))
           (LE: NOmega.le (NOnum i) (trace_length tr)),
@@ -709,23 +828,23 @@ assert (forall i (GE: i >= (extra_write_pos + 1))
   { ins. destruct (states i) as [wp rp ups downs mem bufs]. simpl in *. red.
     destruct (bufs thread) as [| (loc, val) buf'] eqn:BUFS; [simpl in H0; lia| ].
     exists (mkState wp rp ups downs (upd mem loc val) (upd bufs thread buf')). by eapply cpu_propagate. }
-  simpl in BUF_SIZE. cut (count_upto (cpu_write' ∩₁ in_thread thread) i > count_upto (is_cpu_prop ∩₁ in_thread thread) i); [ins; lia| ].
+  simpl in BUF_SIZE. cut (count_upto (cpu_write' ∩₁ in_cpu_thread thread) i > count_upto (is_cpu_prop ∩₁ in_cpu_thread thread) i); [ins; lia| ].
   unfold gt.
   apply Nat.le_lt_trans with (m := n_props).
-  { forward eapply (count_le_filter tr (is_cpu_prop ∩₁ in_thread thread) i def_lbl) as COUNT_LE_FILTER; auto.
+  { forward eapply (count_le_filter tr (is_cpu_prop ∩₁ in_cpu_thread thread) i def_lbl) as COUNT_LE_FILTER; auto.
     rewrite <- Heqlen_props in COUNT_LE_FILTER. simpl in COUNT_LE_FILTER.
     by unfold count_upto. }
-  apply Nat.lt_le_trans with (m := count_upto (cpu_write' ∩₁ in_thread thread) (extra_write_pos + 1)).
+  apply Nat.lt_le_trans with (m := count_upto (cpu_write' ∩₁ in_cpu_thread thread) (extra_write_pos + 1)).
   2: { apply count_upto_more. lia. }
   rewrite Nat.add_1_r, count_upto_next. rewrite <- COUNT_WRITES.
   rewrite check1; [lia| ].
   unfold trace_labels. rewrite <- MATCH_WRITE.
-  remember (cpu_write' ∩₁ in_thread thread) as F.
+  remember (cpu_write' ∩₁ in_cpu_thread thread) as F.
   remember (trace_nth n_props (trace_filter F tr) def_lbl) as elem. 
   forward eapply (proj1 (trace_in_filter elem F tr)); [| intuition]. 
   subst elem. apply trace_nth_in. vauto. }  
 
-forward eapply (filter_ends tr (is_cpu_prop ∩₁ in_thread thread) def_lbl) as [props_end [DOM NOMORE_PROPS]]. 
+forward eapply (filter_ends tr (is_cpu_prop ∩₁ in_cpu_thread thread) def_lbl) as [props_end [DOM NOMORE_PROPS]]. 
 { by rewrite <- Heqlen_props. }
 set (after_last_prop := max (extra_write_pos + 1) props_end).
 
@@ -776,9 +895,9 @@ Proof.
     unfolder'. intuition. }
   pose proof (reg_write_structure _ W). 
   desc.
-  assert (same_thread (trace_labels w) ≡₁ in_thread thread).
+  assert (same_thread (trace_labels w) ≡₁ in_cpu_thread thread).
   { rewrite H. simpl. unfold same_thread. simpl.
-    unfold in_thread.
+    unfold in_cpu_thread.
     red. split; red; ins; desc; vauto. }
   apply set_extensionality in H0. rewrite H0 in *. 
   pose proof sim_subtraces_conv as TMP. specialize_full TMP.
@@ -829,18 +948,18 @@ Proof.
     red in PROP. rewrite P_DEF in PROP.
     generalize PROP. unfolder'. intuition. }
   red in CORR.
-  assert (same_thread (trace_labels w) = in_thread thread) as RESTR_EQUIV. 
+  assert (same_thread (trace_labels w) = in_cpu_thread thread) as RESTR_EQUIV. 
   { apply set_extensionality. rewrite TLAB. simpl.
-    unfold same_thread, in_thread. simpl. red. splits; red; ins; desc; vauto. }
+    unfold same_thread, in_cpu_thread. simpl. red. splits; red; ins; desc; vauto. }
   rewrite RESTR_EQUIV in CORR.
-  replace (count_upto (is_cpu_prop∩₁ in_thread thread) (p + 1)) with ((count_upto (is_cpu_prop∩₁ in_thread thread) p) + 1) in BUF_SIZE.
+  replace (count_upto (is_cpu_prop∩₁ in_cpu_thread thread) (p + 1)) with ((count_upto (is_cpu_prop∩₁ in_cpu_thread thread) p) + 1) in BUF_SIZE.
   2: { unfold count_upto.
        rewrite Nat.add_1_r with (n := p), seqS, Nat.add_0_l.
        rewrite map_app, filterP_app, length_app. simpl.
        rewrite RESTR_EQUIV in PROP.
-       destruct (excluded_middle_informative ((is_cpu_prop∩₁ in_thread thread) (trace_nth p tr def_lbl))); vauto. }
+       destruct (excluded_middle_informative ((is_cpu_prop∩₁ in_cpu_thread thread) (trace_nth p tr def_lbl))); vauto. }
   rewrite <- CORR in BUF_SIZE.
-  cut (count_upto (cpu_write' ∩₁ in_thread thread) (p + 1) <= count_upto (cpu_write' ∩₁ in_thread thread) w).
+  cut (count_upto (cpu_write' ∩₁ in_cpu_thread thread) (p + 1) <= count_upto (cpu_write' ∩₁ in_cpu_thread thread) w).
   { ins. lia. }
   apply count_upto_more. lia. 
 Qed.
@@ -861,11 +980,11 @@ Proof.
   destruct (constructive_indefinite_description _ _) as [p [PROP CORR]]. simpl.
   pose proof (Nat.lt_trichotomy w p). des; auto.
   { subst. red in PROP. exfalso. 
-    apply fpga_write_structure in f. destruct f as [chan [index [meta H0]]].
+    apply fpga_write_structure in f. destruct f as [chan [loc [val [index [meta H0]]]]].
     rewrite H0 in PROP. red in PROP. desc. vauto. }
   exfalso. rename H into LT. 
-  apply fpga_write_structure in f. destruct f as [chan [index [meta TLAB]]].
-  forward eapply (buffer_size_fpga chan (p + 1)) as BUF_SIZE.
+  apply fpga_write_structure in f. destruct f as [chan [loc [val [index [meta TLAB]]]]].
+  forward eapply (buffer_size_upstream_write chan (p + 1)) as BUF_SIZE.
   { contra GE. forward eapply (proj2 (ge_default p)) as P_DEF. 
     { red. intros. apply GE. simpl. red in H. destruct tr; vauto.
       simpl in *. lia. }
@@ -874,7 +993,7 @@ Proof.
   red in CORR.
   assert (same_chan (trace_labels w) = in_chan chan) as RESTR_EQUIV. 
   { apply set_extensionality. rewrite TLAB. simpl.
-    unfold same_chan, in_thread. simpl. red. splits; red; ins; desc; vauto. }
+    unfold same_chan, in_cpu_thread. simpl. red. splits; red; ins; desc; vauto. }
   rewrite RESTR_EQUIV in CORR.
   replace (count_upto (is_fpga_prop∩₁ in_chan chan) (p + 1)) with ((count_upto (is_fpga_prop ∩₁ in_chan chan) p) + 1) in BUF_SIZE.
   2: { unfold count_upto.
@@ -898,7 +1017,7 @@ Proof.
 Qed.
 
 (* Порядок propagate в основную память *)
-Definition vis (e: Event) :=
+(* Definition vis (e: Event) :=
   match (excluded_middle_informative (is_cpu_wr e)) with
   | left W => write2prop (trace_index e)
   | right _ => match (excluded_middle_informative (is_wr_resp e)) with
@@ -907,45 +1026,8 @@ Definition vis (e: Event) :=
     end
   end. 
 
-Definition vis_lt := is_init × Eninit ∪ ⦗Eninit⦘ ⨾ (fun x y => vis x < vis y) ⨾ ⦗Eninit⦘. 
+Definition vis_lt := is_init × Eninit ∪ ⦗Eninit⦘ ⨾ (fun x y => vis x < vis y) ⨾ ⦗Eninit⦘.  *)
 
-Lemma vis_SPO:
-  strict_partial_order vis_lt. 
-Proof.
-  unfold vis_lt, map_rel. 
-  red. split. 
-  { apply irreflexive_union. split.
-    { red. ins. red in H. desc. by apply (proj1 Eninit_non_init x). }
-    red. ins. apply seq_eqv_lr in H. desc. lia. }
-  apply transitiveI.
-  rewrite seq_union_l. apply inclusion_union_l.
-  { apply inclusion_union_r1_search. red. ins.
-    red in H. desc. red in H. desc.
-    red. red in H0. des.
-    { red in H0. by desc. }
-    apply seq_eqv_lr in H0. by desc. }
-  apply inclusion_union_r2_search.
-  rewrite seq_union_r.
-  rewrite !seqA. arewrite (⦗Eninit⦘ ⨾ is_init × Eninit ⊆ ∅₂).
-  { generalize Eninit_non_init. basic_solver. }
-  rewrite !seq_false_r, union_false_l.
-  hahn_frame_l. hahn_frame_r. rewrite !inclusion_seq_eqv_l.
-  red. ins. red in H. desc. lia. 
-Qed. 
-
-Lemma TI_LE_VIS e (ENINIT: Eninit e): trace_index e <= vis e.
-Proof.
-  unfold vis. simpl.
-  destruct (excluded_middle_informative (is_cpu_wr e)).
-  {
-    apply Nat.lt_le_incl. apply w2p_later_cpu.
-    unfold trace_labels. rewrite trace_index_simpl; auto.
-  }
-  destruct (excluded_middle_informative (is_wr_resp e)).
-  2: { lia. }
-  apply Nat.lt_le_incl. apply w2p_later_fpga.
-  unfold trace_labels. rewrite trace_index_simpl; auto.
-Qed.
 
 Lemma read_resp_to_memread_lemma r
     (* (DOM: NOmega.lt_nat_l w (trace_length tr)) *)
@@ -992,13 +1074,6 @@ Definition read2mem_read (r: nat) :=
 (*     ⟪PROP_BEFORE: ip <= i⟫ /\ *)
 (*     ⟪NTH_THREAD_WRITE:  ⟫ *)
 
-Lemma r_vis e (Rr: is_cpu_rd e): vis e = trace_index e.
-Proof.
-  unfold vis.
-  generalize Rr. unfolder'. destruct e; vauto.
-  destruct e; ins.
-  all: destruct (excluded_middle_informative _ ); intuition.
-Qed. 
 
 Definition exact_tid e := match e with
                           | InitEvent _ => 0
@@ -1028,6 +1103,55 @@ Definition vis' (e: Event) :=
   end. 
 
 Definition vis_lt' := is_init × Eninit ∪ ⦗Eninit⦘ ⨾ (fun x y => vis' x < vis' y) ⨾ ⦗Eninit⦘. 
+
+Lemma r_vis e (Rr: is_cpu_rd e): vis' e = trace_index e.
+Proof.
+  unfold vis'.
+  generalize Rr. unfolder'. destruct e; vauto.
+  destruct e; ins.
+  all: destruct (excluded_middle_informative _ ); intuition.
+Qed. 
+
+Lemma vis_SPO:
+  strict_partial_order vis_lt'. 
+Proof.
+  unfold vis_lt', map_rel. 
+  red. split. 
+  { apply irreflexive_union. split.
+    { red. ins. red in H. desc. by apply (proj1 Eninit_non_init x). }
+    red. ins. apply seq_eqv_lr in H. desc. lia. }
+  apply transitiveI.
+  rewrite seq_union_l. apply inclusion_union_l.
+  { apply inclusion_union_r1_search. red. ins.
+    red in H. desc. red in H. desc.
+    red. red in H0. des.
+    { red in H0. by desc. }
+    apply seq_eqv_lr in H0. by desc. }
+  apply inclusion_union_r2_search.
+  rewrite seq_union_r.
+  rewrite !seqA. arewrite (⦗Eninit⦘ ⨾ is_init × Eninit ⊆ ∅₂).
+  { generalize Eninit_non_init. basic_solver. }
+  rewrite !seq_false_r, union_false_l.
+  hahn_frame_l. hahn_frame_r. rewrite !inclusion_seq_eqv_l.
+  red. ins. red in H. desc. lia. 
+Qed. 
+
+Lemma TI_LE_VIS e (ENINIT: Eninit e): trace_index e <= vis' e.
+Proof.
+  unfold vis'. simpl.
+  destruct (excluded_middle_informative (is_cpu_wr e)).
+  {
+    apply Nat.lt_le_incl. apply w2p_later_cpu.
+    unfold trace_labels. rewrite trace_index_simpl; auto.
+  }
+  destruct (excluded_middle_informative (is_wr_resp e)).
+  { apply Nat.lt_le_incl. apply w2p_later_fpga.
+  unfold trace_labels. rewrite trace_index_simpl; auto. }
+  destruct (excluded_middle_informative (is_rd_resp e)).
+  2: lia.
+  { apply Nat.lt_le_incl. apply w2p_later_cpu.
+  unfold trace_labels. rewrite trace_index_simpl; auto. }
+Qed.
 
 
 Definition rf' w r :=
@@ -1060,10 +1184,10 @@ Proof.
 Qed. *)
 
 Lemma RESTR_EQUIV thread index lbl:
-  same_thread (EventLab (ThreadEvent thread index lbl)) = in_thread thread.
+  same_thread (EventLab (ThreadEvent thread index lbl)) = in_cpu_thread thread.
 Proof.
   ins. apply set_extensionality. 
-  unfold same_thread, in_thread. simpl. red. splits; red; ins; desc; vauto.
+  unfold same_thread, in_cpu_thread. simpl. red. splits; red; ins; desc; vauto.
 Qed. 
     
 Definition G :=
@@ -1075,21 +1199,6 @@ Definition G :=
      fenceonepair := ⦗EG ∩₁ is_fence_req_one⦘ ⨾ req_resp_pair ⨾ ⦗EG ∩₁ is_fence_resp_one⦘;
      fenceallpair := ⦗EG ∩₁ is_fence_req_all⦘ ⨾ req_resp_pair ⨾ ⦗EG ∩₁ is_fence_resp_all⦘
   |}.
-
-
-Lemma no_read_from_future': irreflexive (rf G ⨾ sb G).
-Proof.
-  rewrite rfi_union_rfe.
-  arewrite (rfi G ⊆ sb G).
-  rewrite seq_union_l.
-  apply irreflexive_union.
-  split.
-  { rewrite rewrite_trans.
-    all: admit. }
-  (* доказать, что rfe из разных потоков *)
-
-  
-
 
 Lemma WFG: Wf_fpga G.
 Proof.
@@ -1244,7 +1353,416 @@ vauto.
 Qed.
 
 
-Lemma vis_respects_sb_w: restr_rel is_w (sb G) ⊆ vis_lt.
+Lemma mem_read_from_up_bufs st1 st2 (c: Chan) (x: nat) 
+    (MEM_READ: fpga_mem_read' (trace_labels x)) 
+    (IN_CHAN: in_chan c (trace_labels x))
+    (STEP: TSOFPGA_step st1 (trace_labels x) st2)
+    (IN_TRACE: NOmega.lt_nat_l x (trace_length tr))
+  : length (filter is_read_ups (up_bufs (states x) c)) > 0.
+Proof.
+  unfold in_chan in IN_CHAN.
+  unfold lbl_chan_opt in IN_CHAN. 
+  remember (TSi x IN_TRACE def_lbl) as STEP'.
+  simpl in STEP'.
+  unfold trace_labels in *.
+  unfold fpga_mem_read' in MEM_READ.
+  inv STEP'; desf.
+  simpl.
+  rewrite UPSTREAM.
+  Search (filter _ (_ :: _) = (filter _) ++ (filter _)).
+  assert ((read_up loc, meta) :: up_buf' = ((read_up loc, meta) :: nil) ++ up_buf') by vauto.
+  rewrite H.
+  erewrite filter_app.
+  rewrite length_app.
+  assert (is_read_ups (read_up loc, meta)) by vauto.
+  simpl.
+  lia.
+Qed.
+
+Lemma rd_resp_after_memread rd (EN: Eninit rd) (RD: is_rd_resp rd) : (trace_index rd) > read2mem_read (trace_index rd).
+Proof.
+  unfold read2mem_read.
+  desf.
+  2: { exfalso. apply n. erewrite trace_index_simpl'; vauto. }
+  2: { exfalso. apply n. erewrite trace_index_simpl'; vauto. }
+  destruct (constructive_indefinite_description _); simpl; desf.
+  erewrite trace_index_simpl' in f; eauto.
+  destruct rd; desf.
+  destruct e; desf.
+  erewrite trace_index_simpl' in W_P_CORR; eauto.
+
+  erewrite (count_same_chan_in_chan c) in W_P_CORR.
+  2: { unfold in_chan; ins. }
+  erewrite (count_same_chan_in_chan c) in W_P_CORR.
+  2: { unfold in_chan; ins. }
+  (* Admitted. *)
+
+  assert (NOmega.lt_nat_l x (trace_length tr)) as IN_TR. { 
+    apply not_default_found.
+    intro.
+    unfold def_lbl in H.
+    rewrite H in *.
+    destruct THREAD_PROP; vauto.
+  }
+  erewrite <- (buffer_size_upstream_read) in W_P_CORR.
+  2: { red in IN_TR; ins; destruct (trace_length tr); lia. }
+
+  (* cut (z < x \/ z >= x).
+  2: lia.
+  intro CUT; destruct CUT as [GOOD | GEQ]; auto.
+  exfalso. *)
+  assert (length (filter is_read_ups (up_bufs (states x) c)) > 0).
+  {
+    destruct THREAD_PROP as [MREAD IN_CHAN].
+    eapply mem_read_from_up_bufs; eauto.
+    rewrite trace_index_simpl' in IN_CHAN.
+    2: auto.
+    unfold same_chan in IN_CHAN.
+    unfold lbl_chan_opt in IN_CHAN.
+    destruct IN_CHAN as [IN_CHAN CHAN_SOME].
+    desf.
+    eapply TSi. auto.
+  }
+  remember (trace_index (FpgaEvent (Fpga_read_resp c x0 v) index m)) as z.
+  cut (z > x \/ z <= x).
+  2: lia.
+  intro CUT; destruct CUT as [GOOD | GEQ]; auto.
+  remember (count_upto_more z x (fpga_read_resp' ∩₁ in_chan c) GEQ) as CNT_MORE.
+  lia. 
+Qed.
+
+Lemma rf_same_tid_ext_sb w r (RF: rf G w r) (TID: tid w = tid r) : ext_sb w r.
+Proof.
+  unfold ext_sb.
+  simpl in RF.
+  apply seq_eqv_lr in RF.
+  destruct RF as [Ew [RFwr Er]].
+  unfold rf' in RFwr.
+  destruct Ew, Er.
+  unfold is_w, is_r in *.
+  destruct (state_before_event r) as [wp rp up downs mem bufs].
+  desf.
+  simpl in RFwr.
+  red in RFwr.
+  destruct RFwr as [[LOC [VISLT [EG' TT]]] UNUSED].
+  { split. reflexivity. destruct VISLT as [BAD | VISLT].
+    { destruct BAD. desf. }
+    clear UNUSED.
+    destruct VISLT as [WR [EN1 [RD [VIS EN2]]]]; desf.
+    destruct EN1 as [WREQ ENWR].
+    destruct EN2 as [RDEQ ENRD].
+    unfold vis' in VIS.
+    unfold loc in *.
+    rewrite WREQ in *.
+    rewrite RDEQ in *.
+    desf.
+    remember (ThreadEvent thread0 index (Cpu_store x0 v0)) as wr.
+    remember (ThreadEvent thread0 index0 (Cpu_load x0 v)) as rd.
+    assert (cpu_write' (trace_labels(trace_index wr))) 
+      as CPU. { ins. erewrite trace_index_simpl'; vauto. }
+    remember (w2p_later_cpu (trace_index wr) CPU).
+    assert (trace_index (wr) < trace_index (rd)) by lia.
+    assert ((⦗Eninit⦘ ⨾ ext_sb ⨾ ⦗Eninit⦘) wr rd) as SB'. {
+      eapply tb_respects_sb.
+      apply seq_eqv_lr.
+      split; desf; vauto. }
+    apply seq_eqv_lr in SB'.
+    destruct SB' as [Ex [SBxy Ey]].
+    rename index into wr_i.
+    rename index0 into rd_i.
+    assert (~ is_init wr). { intro. eapply Eninit_non_init; red; eauto. }
+    assert (index wr < index rd) as INDEX_INEQ. { eapply ext_sb_index; eauto. }
+    unfold index in INDEX_INEQ.
+    desf. }
+  2: { destruct RFwr as [[LOC [VISLT [EG' TT]]] UNUSED].
+    clear UNUSED.
+    destruct VISLT as [BAD | VISLT].
+    { destruct BAD; desf. }
+    destruct VISLT as [WR [EN1 [RD [VIS EN2]]]]; desf.
+    destruct EN1 as [WREQ ENWR].
+    destruct EN2 as [RDEQ ENRD].
+    unfold vis' in VIS.
+    unfold loc in *.
+    rewrite WREQ in *.
+    rewrite RDEQ in *.
+    desf.
+    remember (FpgaEvent (Fpga_read_resp c x v) index0 m0) as rd.
+    remember (FpgaEvent (Fpga_write_resp c0 x v0) index m) as wr.
+    assert (fpga_write' (trace_labels(trace_index wr))) 
+      as FPGA. { ins. erewrite trace_index_simpl'; vauto. }
+    remember (w2p_later_fpga (trace_index wr) FPGA).
+    assert (trace_index (wr) < read2mem_read (trace_index rd)) as INEQ by lia.
+    assert (read2mem_read (trace_index rd) < trace_index (rd)) as INEQ'.
+    { apply rd_resp_after_memread; vauto. }
+    assert (trace_index wr < trace_index rd) by lia.
+    rename index into wr_i.
+    rename index0 into rd_i.
+    assert ((⦗Eninit⦘ ⨾ ext_sb ⨾ ⦗Eninit⦘) wr rd) as SB'. {
+      eapply tb_respects_sb.
+      apply seq_eqv_lr.
+      split; desf; vauto. }
+    apply seq_eqv_lr in SB'.
+    destruct SB' as [Ex [SBxy Ey]].
+    assert (index wr < index rd) as INDEX_INEQ. { eapply ext_sb_index; vauto. }
+    unfold index in INDEX_INEQ.
+    desf.
+    }
+  {
+  simpl in RFwr.
+  red in RFwr.
+  destruct RFwr as [[LOC [TRACE_BEFORE [S_TID [EN_WR TT]]]] UNUSED].
+  split; [reflexivity |].
+  remember ((ThreadEvent thread0 index (Cpu_store x0 v0))) as wr.
+  remember ((ThreadEvent thread0 index0 (Cpu_load x v))) as rd.
+
+  assert (same_tid rd wr) by vauto.
+  destruct (excluded_middle_informative (Eninit rd)) as [ENRD | NENRD].
+  2: { exfalso.  
+       unfold trace_before in TRACE_BEFORE.
+       assert (trace_index wr >= 0). { unfold trace_index. desf. lia. }
+       assert (trace_index rd = 0). { unfold trace_index. desf. }
+       lia. }
+  assert ((⦗Eninit⦘ ⨾ ext_sb ⨾ ⦗Eninit⦘) wr rd) as SB'. {
+    eapply tb_respects_sb.
+    apply seq_eqv_lr.
+    repeat split; vauto.
+  }
+  apply seq_eqv_lr in SB'.
+  destruct SB' as [Ex [SBxy Ey]].
+  rename index into wr_i.
+  rename index0 into rd_i.
+  assert (index wr < index rd) as INDEX_INEQ. { eapply ext_sb_index; vauto. }
+  unfold index in INDEX_INEQ; desf.
+  } 
+Qed.
+  
+
+
+Lemma rfe_diff_tid w r (RFE: rfe G w r): tid w <> tid r. 
+Proof.
+  intro.
+  (* destruct w, r; desf. *)
+  unfold rfe in RFE.
+  (* unfold rf, sb in RFE.
+  simpl in RFE. *)
+  destruct RFE as [RF NOT_SB].
+  destruct NOT_SB.
+  unfold sb.
+  apply seq_eqv_lr.
+  assert (ext_sb w r) by (apply rf_same_tid_ext_sb; vauto).
+  simpl.
+  simpl in RF.
+  apply seq_eqv_lr in RF.
+  destruct RF as [[EGW WW] [RF [EGR RR]]].
+  vauto.
+Qed.
+  
+Lemma sb_same_tid w r (SB: sb G w r) (NOT_INIT: Eninit w): tid w = tid r.
+Proof.
+  red in SB.
+  assert (~ is_init w).
+  { intro.
+    eapply Eninit_non_init; red; eauto. }
+  unfold tid.
+  apply seq_eqv_lr in SB.
+  destruct SB as [Ex [SBxy Ey]].
+  unfold ext_sb in SBxy.
+  destruct w, r; desf.
+Qed.
+
+Lemma no_read_from_future': irreflexive (rf G ⨾ sb G).
+Proof.
+  rewrite rfi_union_rfe.
+  arewrite (rfi G ⊆ sb G).
+  rewrite seq_union_l.
+  apply irreflexive_union.
+  split.
+  { rewrite rewrite_trans.
+    apply sb_irr.
+    apply sb_trans.
+  }
+  unfold irreflexive; ins.
+  unfold seq in H.
+  destruct H as [e [RFE SB]].
+  assert (Eninit e). {
+    destruct RFE as [RF NSB].
+    destruct RF as [A [B [C [D IS_R]]]].
+    destruct IS_R as [EQ [EG IS_R]].
+    subst.
+    unfold is_r in *.
+    destruct EG; destruct e; desf.
+  }
+  apply rfe_diff_tid in RFE.
+  apply sb_same_tid in SB; vauto.
+  symmetry in SB; auto.
+Qed.
+
+Lemma read_source r (Er: EG r) (Rr: is_r r):
+  exists! w, rf G w r.
+Proof.
+  cut ((exists! w, (EG ∩₁ is_w) w /\ rf' w r) /\ (EG ∩₁ is_r) r).
+  { ins. unfold unique in H. desc.
+    exists x. red. splits.
+    { apply seq_eqv_lr. splits; auto. }
+    ins. desc. apply seq_eqv_lr in H3. desc. apply H1. splits; auto. }
+  split; [| vauto].
+  unfold rf'.
+  do 2 red in Er. des.
+  { exfalso. eapply init_non_r; eauto. }
+  (* red in Er. pose proof Er as Er_.  *)
+  (* apply trace_in_nth with (d := def_lbl) in Er. desc. *)
+  unfold state_before_event.
+  forward eapply (TSi (trace_index r)) with (d := def_lbl) as TSi; eauto.
+  { contra GE.
+    pose proof (proj2 (ge_default (trace_index r)) GE).
+    unfold def_lbl in H. by rewrite trace_index_simpl' in H; vauto. }
+  
+  rewrite trace_index_simpl in TSi; auto.
+  destruct r; vauto. 
+  remember (ThreadEvent thread index e) as r.
+  (* destruct (bufs thread) eqn:BUF. *)
+  remember (states (trace_index r)) as st. destruct st as [wp rp ups downs mem bufs].
+  destruct (filter (fun loc_val : Loc * Val => fst loc_val =? loc r) (bufs thread)) eqn:BUF.
+  { remember (fun e : Event => loc e = loc r /\ vis_lt e r /\ EG e /\ is_w e) as writes.
+    cut (exists! w, latest_of_by writes (co G) w).
+    {
+      subst writes. intros [w [LATEST UNIQ]]. red in LATEST. desc.
+      exists w.
+      red.
+      assert (exact_tid r = thread) as TID_E. by desf.
+      rewrite <- TID_E in BUF.
+      rewrite BUF.
+      destruct excluded_middle_informative as [CPU_W | NOT_CPU_W].
+      { split.
+        { split; vauto.
+          red. splits; vauto. intros. specialize (LATEST0 y S').
+          red in LATEST0. des; [vauto| ]. simpl in LATEST0. apply seq_eqv_lr in LATEST0. desc. red in LATEST4. desc. vauto. }
+      ins. desc. red in H0. desc. apply UNIQ. red. splits; vauto.
+      ins. specialize (H1 y S').
+      red in H1. des; [vauto| ].
+      red. right. apply seq_eqv_lr. splits; vauto.
+      red. split; auto. congruence. }
+    apply latest_unique.
+    { apply antisymmetric_inclusion with (r := co G); [| basic_solver].
+      apply strict_partial_order_antisymmetric.
+      by destruct (co_loc_total (loc r)). }
+    assert (set_finite writes) as WRITES_FIN.
+    { arewrite (writes ⊆₁ fun e => loc e = loc r /\ vis_lt e r) by basic_solver.
+      pose proof (fsupp_vis_loc r) as [findom FINDOM].
+      red. exists findom. ins. desc. apply FINDOM. red. split; auto. }
+    assert (~ writes ≡₁ ∅) as HAS_WRITES.
+    { apply set_nonemptyE. exists (InitEvent (loc r)).
+      subst. splits; vauto. }
+    assert (strict_total_order writes (co G)) as TOTAL.
+    { red. split.
+      { by destruct (co_loc_total (loc r)). }
+      forward eapply (@is_total_mori _ (EG ∩₁ is_w ∩₁ (fun a => loc a = loc r)) writes) as H.
+      { subst. unfold Basics.flip. basic_solver. }
+      { eapply (inclusion_refl2 (co G)). }
+      apply H, co_loc_total. }
+    apply latest_fin; eauto. }
+  remember (fun e : Event => loc e = loc r /\ trace_before e r /\ exact_tid e = thread /\  Eninit e /\ is_w e) as writes.
+  cut (exists w, unique (latest_of_by writes trace_before) w).
+  { ins. unfold unique in H. desc. red in H. desc.
+    rewrite Heqwrites in H. desc.
+    exists w. red. splits; vauto.
+    ins. desc. red in H6. desc. apply H0. red. splits; vauto. }
+
+  assert (set_finite writes) as WRITES_FIN.
+  { apply set_finite_mori with (x := fun e => trace_before e r /\ Eninit e).
+    { red. rewrite Heqwrites. basic_solver. }
+    red.
+    set (extract_event := fun i => match (trace_labels i) with
+                                | inr _ => InitEvent 0
+                                | inl e => e
+                                end).
+    exists (map extract_event (List.seq 0 (trace_index r))).
+    ins. desc.
+    replace x with (extract_event (trace_index x)).
+    2: { unfold extract_event.
+         unfold trace_labels. by rewrite trace_index_simpl. }
+    apply in_map. by apply in_seq0_iff. }
+  assert (~ writes ≡₁ ∅) as HAS_WRITES.
+  { red. ins.
+    forward eapply (@no_writes_no_buffer thread (loc r) (trace_index r)) as BUF_EMPTY; eauto.
+    { contra GE. forward eapply (proj2 (ge_default (trace_index r))); auto.
+      unfold trace_labels. rewrite trace_index_simpl, Heqr; auto. by unfolder'. }
+    { ins. red. ins. desc.
+      apply le_lt_or_eq in H2. des.
+      2: { unfold write2prop in H2. destruct (excluded_middle_informative _).
+           2: { lia. }
+           destruct (constructive_indefinite_description _ _). simpl in *. desc.
+           subst. rewrite trace_index_simpl' with (e := ThreadEvent _ _ _) in THREAD_PROP; auto.
+           generalize THREAD_PROP. unfolder'. intuition. }
+      apply (proj1 H e). rewrite Heqwrites. splits; auto. }
+    simpl in BUF_EMPTY. rewrite <- Heqst in BUF_EMPTY. simpl in BUF_EMPTY.
+    by rewrite BUF in BUF_EMPTY. }
+  assert (strict_total_order writes trace_before) as TOTAL.
+  { cdes tb_SPO.
+    red. split; auto.
+    forward eapply (@is_total_mori _ Eninit writes) as H.
+    { red. basic_solver. }
+    { eapply (inclusion_refl2 trace_before). }
+      by apply H. }
+  forward eapply (@latest_fin _ _ trace_before WRITES_FIN HAS_WRITES) as LATEST'; [vauto| ].
+  apply latest_unique in LATEST'.
+  2: { apply antisymmetric_inclusion with (r := trace_before); [| basic_solver].
+       apply strict_partial_order_antisymmetric. by cdes tb_SPO. }
+  unfold unique in LATEST'. desc. exists x. split; [vauto| ].
+  red in LATEST'. desc. by rewrite Heqwrites in LATEST'. 
+Qed. 
+
+
+(* Well formed *)
+
+Lemma G_well_formed: Wf G.
+Proof.
+  split.
+  pose proof WF as WF'.
+  destruct WF'.
+  { ins. desc. do 2 red in H. des; [vauto|].
+    assert (~ is_init b).
+    { destruct a, b; vauto. }
+    do 2 red in H0. des; [vauto|].
+    destruct a, b; vauto.
+    3: { exfalso. by simpl in H3. }
+
+    { red in H2. simpl in H2. subst index0.
+    red in H, H0. apply trace_in_nth with (d := def_lbl) in H. apply trace_in_nth with (d := def_lbl) in H0. desc.
+    simpl in *. red in TSO_TR_WF.
+    specialize TSO_TR_WF with (d := def_lbl) (thread := thread0) (index1 := index) (index2 := index). 
+    pose proof (Nat.lt_trichotomy n n0). des.
+    2: { subst. congruence. }
+    all: subst; specialize_full TSO_TR_WF; eauto; lia. }
+
+    red in H2. simpl in H2. subst index0.
+    red in H, H0. apply trace_in_nth with (d := def_lbl) in H. apply trace_in_nth with (d := def_lbl) in H0. desc.
+    simpl in *. red in FPGA_TR_WF.
+    pose proof (Nat.lt_trichotomy n n0). des.
+    2: { subst. congruence. }
+    { specialize FPGA_TR_WF with (d := def_lbl) (index1 := index) (index2 := index) (meta1 := m0) (meta2 := m). 
+      subst; specialize_full FPGA_TR_WF; eauto; lia. }
+    { specialize FPGA_TR_WF with (d := def_lbl) (index1 := index) (index2 := index) (meta1 := m) (meta2 := m0). 
+      subst; specialize_full FPGA_TR_WF; eauto; lia. }}
+  { simpl. basic_solver. }
+  { simpl. basic_solver. }
+  { simpl. rewrite inclusion_seq_eqv_r, inclusion_seq_eqv_l.
+    unfold rf'. red. ins. desf.
+    3: { unfold latest_of_by in H. by desc. }
+    all: destruct (state_before_event y); destruct (filter _ _); unfold latest_of_by in H; by desc. }
+  { admit. }
+  { unfold functional. intros r w1 w2 RF1 RF2. unfold transp in *.
+    forward eapply (@read_source r) as [w' [RF' UNIQ]]. 
+    1, 2: generalize RF1; simpl; basic_solver.
+    rewrite <- (UNIQ w1), <- (UNIQ w2); [auto|generalize RF2 |generalize RF1]; simpl; basic_solver. }
+
+  Admitted.
+
+
+
+(* \\Well formed *)
+
+Lemma cpu_vis_respects_sb_w: restr_rel (is_cpu ∩₁ is_w) (sb G) ⊆ vis_lt.
 Proof.
 unfold restr_rel. red. ins. destruct H as [SBxy [Wx Wy]].
 destruct (vis_lt_init_helper x y SBxy) as [|[E'x E'y]]; auto. 
@@ -1275,15 +1793,15 @@ destruct (excluded_middle_informative _) as [X | X].
     destruct (constructive_indefinite_description _ _) as [py Py].
     simpl in *. desc.
     unfold trace_labels in *. rewrite !trace_index_simpl in *; auto.
-    assert (exists thread, same_thread (EventLab x) = in_thread thread /\ same_thread (EventLab y) = in_thread thread).
+    assert (exists thread, same_thread (EventLab x) = in_cpu_thread thread /\ same_thread (EventLab y) = in_cpu_thread thread).
     { pose proof (reg_write_structure _ c). desc. inv H. 
       pose proof (reg_write_structure _ c0). desc. inv H0. 
       red in TIDxy. simpl in TIDxy. inv TIDxy.
       exists thread0. 
       split; apply RESTR_EQUIV. }
     desc. rewrite H, H0 in *. 
-    assert (count_upto (cpu_write' ∩₁ in_thread thread) (trace_index x) < count_upto (cpu_write' ∩₁ in_thread thread) (trace_index y)).
-    { subst. apply Nat.lt_le_trans with (m := count_upto (cpu_write' ∩₁ in_thread thread) (trace_index x + 1)).
+    assert (count_upto (cpu_write' ∩₁ in_cpu_thread thread) (trace_index x) < count_upto (cpu_write' ∩₁ in_cpu_thread thread) (trace_index y)).
+    { subst. apply Nat.lt_le_trans with (m := count_upto (cpu_write' ∩₁ in_cpu_thread thread) (trace_index x + 1)).
       2: { eapply count_upto_more. lia. }
       rewrite Nat.add_1_r, count_upto_next.
       rewrite check1; [lia|].
@@ -1293,132 +1811,16 @@ destruct (excluded_middle_informative _) as [X | X].
     } 
     apply lt_diff in H1. desc. rewrite W_P_CORR0, W_P_CORR in H1. 
     destruct (NPeano.Nat.lt_ge_cases px py); auto. 
-    remember (count_upto_more py px (is_cpu_prop ∩₁ in_thread thread) H2); lia. }
-  destruct (NPeano.Nat.lt_ge_cases (write2prop (trace_index x)) (trace_index y)) as [LL | LE].
-  exfalso.
-  forward eapply (@reg_write_structure (EventLab x)) as H. 
-  { vauto. }
-  desc. inversion H. clear H.  
-  destruct y.
-  { exfalso. by apply (proj1 Eninit_non_init (InitEvent x0)). }
-  destruct l; vauto.
-  assert (thread0 = thread); [|subst thread0]. 
-  { red in TIDxy. vauto. }
-  remember (ThreadEvent thread index0 (Armw x0 vr vw)) as tlab. 
-  assert (NOmega.lt_nat_l (trace_index tlab) (trace_length tr)) as DOM. 
-  { contra GE. apply ge_default in GE.
-    unfold trace_labels in GE. rewrite trace_index_simpl in GE; auto. 
-    rewrite Heqtlab in GE. discriminate GE. }
-  set (st := states (trace_index tlab)).
-  forward eapply (TSi (trace_index tlab)) with (d := def_lbl) as TSi; eauto. 
-  rewrite trace_index_simpl in TSi; auto.
-  rewrite Heqtlab in TSi at 2. inversion TSi. subst. 
-  remember (ThreadEvent thread index0 (Armw x0 (sh_mem x0) vw)) as e_rmw. 
-  remember (ThreadEvent thread index (Astore loc val)) as e_w.
-  forward eapply (@buffer_size thread (trace_index e_rmw)) as BUF_SIZE. 
-  { destruct (trace_length tr); auto. simpl in *. lia. }
-  simpl in BUF_SIZE. rewrite <- H0 in BUF_SIZE. simpl in BUF_SIZE.
-  rewrite NO_BUF in BUF_SIZE. simpl in BUF_SIZE. rewrite Nat.add_0_r in BUF_SIZE.
-  remember (write2prop (trace_index e_w)) as vis_w. 
-  assert (count_upto (regular_write' ∩₁ same_thread (trace_labels (trace_index e_w))) (trace_index e_w) =
-          count_upto (is_prop ∩₁ same_thread (trace_labels (trace_index e_w))) vis_w) as VIS_W.
-  { subst vis_w. unfold write2prop in *. destruct (excluded_middle_informative _).
-    2: { generalize n, X. rewrite trace_index_simpl'; auto. by unfolder'. }
-    destruct (constructive_indefinite_description _ _). desc. simpl in *.
-    lia. }
-  replace (same_thread (trace_labels (trace_index e_w))) with (in_thread thread) in VIS_W.
-  2: { rewrite trace_index_simpl'; auto. subst e_w. by rewrite RESTR_EQUIV. }
-  assert (count_upto (regular_write' ∩₁ in_thread thread) (trace_index e_w) < count_upto (regular_write' ∩₁ in_thread thread) (trace_index e_rmw)) as MORE_WRITES.
-  { unfold lt. rewrite <- Nat.add_1_r.
-    rewrite <- (@check1 _ (regular_write' ∩₁ in_thread thread) (trace_labels ((trace_index e_w)))).
-    2: { red. rewrite trace_index_simpl'; auto. by subst e_w. }
-    rewrite <- count_upto_next. apply count_upto_more. lia. }
-  assert (count_upto (is_prop ∩₁ in_thread thread) (trace_index e_rmw) <= count_upto (is_prop ∩₁ in_thread thread) vis_w) as MORE_PROPS.
-  { apply count_upto_more. lia. }
-  lia. 
-}
-destruct (excluded_middle_informative _) as [X | X]; destruct (excluded_middle_informative _) as [X' | X']; auto. 
-3: { apply lt_trans with (m := trace_index y); auto. apply w2p_later.
-      unfold trace_labels. rewrite trace_index_simpl; auto. }
-{ unfold write2prop. destruct (excluded_middle_informative _); vauto.
-  2: { unfold trace_labels in n. rewrite trace_index_simpl in n; vauto. }
-  destruct (excluded_middle_informative _); vauto.
-  2: { unfold trace_labels in n. rewrite trace_index_simpl in n; vauto. }
-  destruct (constructive_indefinite_description _ _) as [px Px].
-  destruct (constructive_indefinite_description _ _) as [py Py].
-  simpl in *. desc.
-  unfold trace_labels in *. rewrite !trace_index_simpl in *; auto.
-  assert (exists thread, same_thread (inl x) = in_thread thread /\ same_thread (inl y) = in_thread thread).
-  { pose proof (reg_write_structure _ r). desc. inv H. 
-    pose proof (reg_write_structure _ r0). desc. inv H0. 
-    red in TIDxy. simpl in TIDxy. inv TIDxy.
-    exists thread0. 
-    split; apply RESTR_EQUIV. }
-  desc. rewrite H, H0 in *. 
-  assert (count_upto (regular_write' ∩₁ in_thread thread) (trace_index x) < count_upto (regular_write' ∩₁ in_thread thread) (trace_index y)).
-  { subst. apply Nat.lt_le_trans with (m := count_upto (regular_write' ∩₁ in_thread thread) (trace_index x + 1)).
-    2: { eapply count_upto_more. lia. }
-    rewrite Nat.add_1_r, count_upto_next.
-    rewrite check1; [lia|].
-    unfold trace_labels. rewrite trace_index_simpl; auto. red. split; auto.
-    rewrite <- H. unfold same_thread. generalize r. destruct x. unfolder'. intuition. vauto. } 
-  apply lt_diff in H1. desc. rewrite W_P_CORR0, W_P_CORR in H1. 
-  destruct (NPeano.Nat.lt_ge_cases px py); auto. 
-  pose proof (count_upto_more (is_prop ∩₁ in_thread thread) H2). lia. }
-destruct (NPeano.Nat.lt_ge_cases (write2prop (trace_index x)) (trace_index y)) as [| LE]; auto.
-exfalso.
-forward eapply (@reg_write_structure (inl x)) as H. 
-{ vauto. }
-desc. inversion H. clear H.  
-destruct y.
-{ exfalso. by apply (proj1 Eninit_non_init (InitEvent x0)). }
-destruct l; vauto.
-assert (thread0 = thread); [|subst thread0]. 
-{ red in TIDxy. vauto. }
-remember (ThreadEvent thread index0 (Armw x0 vr vw)) as tlab. 
-assert (NOmega.lt_nat_l (trace_index tlab) (trace_length tr)) as DOM. 
-{ contra GE. apply ge_default in GE.
-  unfold trace_labels in GE. rewrite trace_index_simpl in GE; auto. 
-  rewrite Heqtlab in GE. discriminate GE. }
-set (st := states (trace_index tlab)).
-forward eapply (TSi (trace_index tlab)) with (d := def_lbl) as TSi; eauto. 
-rewrite trace_index_simpl in TSi; auto.
-rewrite Heqtlab in TSi at 2. inversion TSi. subst. 
-remember (ThreadEvent thread index0 (Armw x0 (sh_mem x0) vw)) as e_rmw. 
-remember (ThreadEvent thread index (Astore loc val)) as e_w.
-forward eapply (@buffer_size thread (trace_index e_rmw)) as BUF_SIZE. 
-{ destruct (trace_length tr); auto. simpl in *. lia. }
-simpl in BUF_SIZE. rewrite <- H0 in BUF_SIZE. simpl in BUF_SIZE.
-rewrite NO_BUF in BUF_SIZE. simpl in BUF_SIZE. rewrite Nat.add_0_r in BUF_SIZE.
-remember (write2prop (trace_index e_w)) as vis_w. 
-assert (count_upto (regular_write' ∩₁ same_thread (trace_labels (trace_index e_w))) (trace_index e_w) =
-        count_upto (is_prop ∩₁ same_thread (trace_labels (trace_index e_w))) vis_w) as VIS_W.
-{ subst vis_w. unfold write2prop in *. destruct (excluded_middle_informative _).
-  2: { generalize n, X. rewrite trace_index_simpl'; auto. by unfolder'. }
-  destruct (constructive_indefinite_description _ _). desc. simpl in *.
-  lia. }
-replace (same_thread (trace_labels (trace_index e_w))) with (in_thread thread) in VIS_W.
-2: { rewrite trace_index_simpl'; auto. subst e_w. by rewrite RESTR_EQUIV. }
-assert (count_upto (regular_write' ∩₁ in_thread thread) (trace_index e_w) < count_upto (regular_write' ∩₁ in_thread thread) (trace_index e_rmw)) as MORE_WRITES.
-{ unfold lt. rewrite <- Nat.add_1_r.
-  rewrite <- (@check1 _ (regular_write' ∩₁ in_thread thread) (trace_labels ((trace_index e_w)))).
-  2: { red. rewrite trace_index_simpl'; auto. by subst e_w. }
-  rewrite <- count_upto_next. apply count_upto_more. lia. }
-assert (count_upto (is_prop ∩₁ in_thread thread) (trace_index e_rmw) <= count_upto (is_prop ∩₁ in_thread thread) vis_w) as MORE_PROPS.
-{ apply count_upto_more. lia. }
-lia. 
+    remember (count_upto_more py px (is_cpu_prop ∩₁ in_cpu_thread thread) H2); lia. }
+  destruct Wx.
+  unfold is_cpu, is_cpu_wr, is_w in *.
+  unfolder'.
+  desf.
 Qed.
 
 Lemma Ax86ConsistentG: Ax86Consistent G.
 Proof.
-  split.
-  {
-    red. red.
-    ins.
-    destruct H.
-    { admit. }
-    
-  }
+  Admitted.
 
 Lemma TSO_op_implies_decl:
   (fun e => trace_elems tr (EventLab e)) ≡₁ acts G \₁ is_init /\ 
